Changed CIH, much progress on ITreeDijkstra.

extra/Dijkstra/ITreeDijkstra.v
@@ -22,6 +22,26 @@ Import MonadNotation.
 #[local] Open Scope monad_scope.
 #[local] Open Scope delayspec_scope.
 
+  #[local] Tactic Notation "step" :=
+  match goal with 
+  | |- context [@body _] => step 
+  | |- context [@elem _] => step 
+  | |- _ => (* gfp case *) repeat red; step 
+  end.
+
+#[local] Tactic Notation "step" "in" ident(h) :=
+  repeat red in h; step in h;
+  match type of h with
+  | context [@body _] => repeat red in h
+  | _ => idtac
+  end.
+
+#[local] Tactic Notation "coinduction" simple_intropattern(c)
+  simple_intropattern(CIH) := 
+  repeat red; coinduction c CIH. 
+
+
+
 Section ITreeDijkstra.
 
   Context (E : Type -> Type).
@@ -100,7 +120,7 @@ Section ITreeDijkstra.
     (*bind_ret*)
     repeat red. cbn. intros. split; intros; basic_solve.
     - apply invert_ret in H. subst. auto.
-    - pinversion H.
+    - sinv H.
     - left. exists x. split; auto. constructor. reflexivity.
   Qed.
   Next Obligation.
@@ -239,11 +259,11 @@ Section ITreeDijkstra.
   Instance bisim_equiv {A} : Equivalence (@bisim A).
   Proof.
     constructor; red.
-    - unfold bisim. coinduction c cih. intros. cbn; red. destruct (observe_stream x); auto with itree.
-    - unfold bisim at -1. coinduction c cih. intros.
+    - coinduction c CIH. intros. cbn; red. destruct (observe_stream x); auto with itree.
+    - coinduction c CIH. intros.
       cbn; red.
       red in H; sinv H; auto with itree.
-    - unfold bisim at 3. coinduction c cih. intros. cbn; red.
+    - unfold bisim at 3. coinduction c CIH. intros. cbn; red.
       red in H; sinv H; red in H0; sinv H0; auto with itree.
       + rewrite <- H in H3. discriminate.
       + rewrite <- H2 in H4. discriminate.
@@ -251,24 +271,34 @@ Section ITreeDijkstra.
         constructor. eauto.
    Qed.
 
+(* step notes: 
+step on elem should not reduce 
+step on mon can reduce 
+step on gfp can reduce. 
+*)
+
   Instance proper_bisim_app {A} : Proper (@bisim A ==> bisim ==> bisim) app.
   Proof.
-    repeat red. coinduction c cih. intros s1 s2 H12 s3 s4 H34.
-     cbn; red. unfold app. pinversion H12.
-    - simpl. destruct s3. destruct s4. pinversion H34; simpl in *; subst; auto with itree.
-      constructor. left. apply pacobot2. auto.
-    - cbn. constructor. right. apply CIH; auto.
+     coinduction c CIH. intros s1 s2 H12 s3 s4 H34.
+     cbn; red. unfold app. sinv H12.
+    - simpl. destruct s3. destruct s4. sinv H34; simpl in *; subst; auto with itree.
+      constructor. now do 2 step. 
+    - cbn. constructor. apply CIH; auto.
   Qed.
 
-  Instance proper_bisim_inf_imp {A} : Proper (@bisim A ==> impl) is_inf.
+
+
+#[local] Tactic Notation "icbn" := repeat red; cbn.  
+
+  Instance proper_bisim_inf_imp {A} : Proper (@bisim A ==> Basics.impl) is_inf.
   Proof.
-    repeat red. pcofix CIH.
-    intros s1 s2 H12 H. pfold. red. punfold H. red in H.
-    punfold H12. red in H12. inversion H12; subst; auto.
-    - rewrite <- H1 in H. inversion H.
-    - inversion H. subst. pclearbot.
-      constructor. right. eapply CIH; eauto.
-      rewrite <- H3 in H0. injection H0 as H0 . subst. auto.
+    coinduction c CIH.
+    intros s1 s2 H12 H. icbn. step in H. 
+    step in H12. inv H12. 
+    - rewrite <- H1 in H. inv H.
+    - inversion H; subst. 
+      constructor. eapply CIH; eauto.
+      rewrite <- H3 in H0. inv H0.
   Qed.
 
   Instance proper_bisim_inf {A} : Proper (@bisim A ==> iff) (is_inf).
@@ -279,9 +309,9 @@ Section ITreeDijkstra.
 
   Lemma app_inf : forall (A : Type) (s1 s2 : stream A), is_inf s1 -> bisim (app s1 s2) s1.
   Proof.
-    intros A. pcofix CIH. intros s1 s2 Hinf. pfold. unfold app.
-    pinversion Hinf.
-    red. cbn. rewrite <- H. constructor. right. apply CIH; auto.
+    intros A. coinduction c CIH. intros s1 s2 Hinf. icbn. unfold app.
+    sinv Hinf.
+    cbn. constructor. apply CIH; auto.
   Qed.
 
   Variant forall_streamF {A : Type} (P : A -> Prop) (F : stream A -> Prop) : stream' A -> Prop :=
@@ -293,14 +323,15 @@ Section ITreeDijkstra.
   Definition forall_stream_ {A : Type} (P : A -> Prop) (F : stream A -> Prop) : stream A -> Prop :=
     fun s => forall_streamF P F (observe_stream s).
 
-  Lemma forall_stream_monot (A : Type) (P : A -> Prop) : monotone1 (forall_stream_ P).
+  Lemma forall_stream_mono (A : Type) (P : A -> Prop) : Proper (leq ==> leq) (forall_stream_ P).
   Proof.
-    red. intros. red. red in IN. destruct IN; auto with itree.
+    repeat red. intros. red in H0. destruct H0; auto with itree.
+    constructor; auto. now apply H. 
   Qed.
 
-  Hint Resolve forall_stream_monot : paco.
+  Definition forall_stream_mon A P := Build_mon (forall_stream_mono A P). 
 
-  Definition forall_stream {A : Type} (P : A -> Prop) := paco1 (forall_stream_ P) bot1.
+  Definition forall_stream {A : Type} (P : A -> Prop) := gfp (forall_stream_mon A P).
 
   Inductive inf_manyF {A : Type} (P : A -> Prop) (F : stream A -> Prop) : stream' A -> Prop :=
     | cons_search (h : A) (t : stream A) : inf_manyF P F (observe_stream t) -> inf_manyF P F (ConsF h t)
@@ -312,33 +343,34 @@ Section ITreeDijkstra.
   Definition inf_many_ {A : Type} (P : A -> Prop) (F : stream A -> Prop) : stream A -> Prop :=
     fun s => inf_manyF P F (observe_stream s).
 
-  Lemma inf_many_monot (A : Type) (P : A -> Prop) : monotone1 (inf_many_ P).
+  Lemma inf_many_mono (A : Type) (P : A -> Prop) : Proper (leq ==> leq) (inf_many_ P).
   Proof.
-    red. intros. red in IN. red. induction IN; auto with itree.
+    repeat red. intros. red in H0. induction H0; auto with itree.
+    apply cons_found; auto. now apply H. 
   Qed.
 
-  Hint Resolve inf_many_monot : paco.
+  Definition inf_many_mon A P := Build_mon (inf_many_mono A P). 
 
-  Definition inf_many {A : Type} (P : A -> Prop) := paco1 (inf_many_ P) bot1.
+  Definition inf_many {A : Type} (P : A -> Prop) := gfp (inf_many_mon A P).
 
   Lemma inf_many_inf : forall (A : Type) (P : A -> Prop) (s : stream A),
       inf_many P s -> is_inf s.
   Proof.
-    intros A P. pcofix CIH. intros s Him.
-    punfold Him. red in Him. pfold. red.
-    induction Him; auto with itree. pclearbot.
-    auto with itree.
+    intros A P. coinduction c CIH. intros s Him.
+    step in Him. icbn. 
+    induction Him; auto with itree.
+    constructor. apply CIH. now step. 
   Qed.
 
   Lemma inf_and_forall : forall (A : Type) (P : A -> Prop) (s : stream A),
       is_inf s -> forall_stream P s -> inf_many P s.
   Proof.
-    intros A P. pcofix CIH. intros s Hinf Hforall.
-    pfold. red. punfold Hinf. red in Hinf. punfold Hforall.
-    red in Hforall. inversion Hinf.
-    inversion Hforall.
+    intros A P. coinduction c CIH. intros s Hinf Hforall.
+    icbn. step in Hinf. step in Hforall.
+    inv Hinf.
+    inv Hforall.
     - rewrite <- H in H2. discriminate.
-    - pclearbot. rewrite <- H in H1. injection H1 as H1. subst.
+    - rewrite <- H in H1. inv H1.
       apply cons_found; auto.
   Qed.
 
@@ -347,7 +379,6 @@ Section ITreeDijkstra.
   (*need a way to relate trees across event types if they never use it*)
 
   Definition rel_eventless {E1 E2 R} (t1 : itree E1 R) (t2 : itree E2 R) : Prop := False.
-
   Inductive eqitEF {E1 E2 : Type -> Type} {R1 R2 : Type} (RR : R1 -> R2 -> Prop)
             (sim : itree E1 R1 -> itree E2 R2 -> Prop) : itree' E1 R1 -> itree' E2 R2 -> Prop :=
     | EqERet : forall r1 r2, RR r1 r2 -> eqitEF RR sim (RetF r1) (RetF r2)
@@ -368,15 +399,16 @@ Section ITreeDijkstra.
              (t1 : itree E1 R1) (t2 : itree E2 R2)
     := eqitEF RR sim (observe t1) (observe t2).
 
-  Definition eqitE {E1 E2} {R1 R2} RR := paco2 (eqitE_ E1 E2 R1 R2 RR) bot2.
+  Lemma eqitE_mono {E1 E2 R1 R2 RR} : Proper (leq ==> leq)  (@eqitE_ E1 E2 R1 R2 RR).
+    Proof.
+      repeat red. intros. rename x into t1. rename y into t2.
+      induction H0; eauto with itree.
+      constructor. now apply H. 
+    Qed.
 
-  Lemma eqitE_monot {E1 E2 R1 R2 RR} : monotone2  (@eqitE_ E1 E2 R1 R2 RR).
-  Proof.
-    repeat red. intros. rename x0 into t1. rename x1 into t2.
-    induction IN; eauto with itree.
-  Qed.
+  Definition eqitE_mon {E1 E2 R1 R2 RR} := Build_mon (@eqitE_mono E1 E2 R1 R2 RR).
 
-  Hint Resolve eqitE_monot : paco.
+  Definition eqitE {E1 E2} {R1 R2} RR := gfp (@eqitE_mon E1 E2 R1 R2 RR).
 
   Definition equivE {E1 E2} {R} : itree E1 R -> itree E2 R -> Prop := eqitE eq.
 
@@ -390,35 +422,33 @@ Section ITreeDijkstra.
     : itree E R -> Prop := fun t => eventlessF F (observe t).
 
   Hint Unfold eventless_ : itree.
-
-  Definition eventless {E : Type -> Type} {R : Type} : itree E R -> Prop :=
-    paco1 (eventless_) bot1.
-
-  Lemma eventless_monot {E1 R} : monotone1 (@eventless_ E1 R).
+  
+  Lemma eventless_mono {E1 R} : Proper (leq ==> leq) (@eventless_ E1 R).
   Proof.
-    red. intros. red in IN. red. inversion IN; auto with itree.
+    repeat red. intros. red in H0. inversion H0; auto with itree.
+    constructor. now apply H.  
   Qed.
 
-  Hint Resolve eventless_monot : paco.
+  Definition eventless_mon {E1 R} := Build_mon (@eventless_mono E1 R).
 
-  Instance proper_eventless_imp {E1 R} : Proper (eutt eq ==> impl) (@eventless E1 R) .
+  Definition eventless {E : Type -> Type} {R : Type} : itree E R -> Prop :=
+    gfp (@eventless_mon E R).
+
+  Instance proper_eventless_imp {E1 R} : Proper (eutt eq ==> Basics.impl) (@eventless E1 R) .
   Proof.
-    repeat red. pcofix CIH.
+    repeat red. coinduction c CIH.
     intros t1 t2 Heutt Hev.
-    pfold. punfold Heutt.  red.
-    unfold_eqit. assert (Hev' : eventless t1); auto. punfold Hev.
+    step in Heutt. icbn.
+    assert (Hev' := Hev). step in Hev.
     dependent induction Heutt; subst; auto with itree.
-    - rewrite <- x. auto with itree.
-    - rewrite <- x. constructor. right. eapply CIH; eauto.
-      specialize (itree_eta t1) as Ht1. rewrite <- x0 in Ht1.
-      rewrite Ht1. rewrite tau_eutt. pclearbot. auto.
-    - red in Hev. inversion Hev; subst.
-      + rewrite <- H0 in x0. discriminate.
-      + rewrite <- H in x0. discriminate.
-    - red in Hev. rewrite <- x in Hev. inversion Hev; subst.
-      pclearbot. eapply IHHeutt; try apply H0; eauto. red.
-      punfold H0.
-    - rewrite <- x. constructor. right. eapply CIH; eauto with itree.
+    - simpobs. auto with itree.
+    - simpobs. constructor. eapply CIH; eauto.
+      inv Hev. 
+    - simpobs. inv Hev. 
+    - simpobs. inv Hev.
+      eapply IHHeutt; try apply H0; eauto.
+      now step in H0. 
+    - simpobs. constructor. unstep in Heutt. eapply CIH; eauto with itree.
   Qed.
 
   Instance proper_eventless {E1 R} : Proper (eutt eq ==> iff) (@eventless E1 R).
@@ -432,42 +462,38 @@ Section ITreeDijkstra.
                  (t1 : itree E1 R1) (t2 : itree E1 R2),
       eventless t1 -> eutt RR t1 t2 -> eqitE RR t1 t2.
   Proof.
-    intros E1 R1 R2 RR. pcofix CIH. intros.
-    punfold H1. unfold_eqit. pfold. red. dependent induction H1; auto.
-    - rewrite <- x0. rewrite <- x. constructor. auto.
-    - rewrite <- x0. rewrite <- x.
-      constructor. right.
+    intros E1 R1 R2 RR. coinduction c CIH. intros.
+    step in H0. icbn. dependent induction H0; auto.
+    - simpobs. eret. 
+    - simpobs.
+      constructor.  
       specialize (itree_eta t1) as Ht1. specialize (itree_eta t2) as Ht2.
-      rewrite <- x0 in Ht1. rewrite <- x in Ht2.
+      simpobs. 
       assert (t1 ≈ m1). { rewrite Ht1. rewrite tau_eutt. reflexivity. }
       assert (t2 ≈ m2). { rewrite Ht2. rewrite tau_eutt. reflexivity. }
-      pclearbot.
       apply CIH; auto.
-      rewrite <- H. auto.
-    - exfalso. pinversion H0.
-      + rewrite <- H1 in x0. discriminate.
-      + rewrite <- H in x0. discriminate.
-    - rewrite <- x. constructor.
-      specialize (itree_eta t1) as Ht1. rewrite <- x in Ht1.
-      rewrite Ht1 in H0. pinversion H0.
-      subst. eapply IHeqitF; try apply H2; eauto.
-    - rewrite <- x. constructor. eapply IHeqitF; eauto.
+      now rewrite <- H0. 
+    - exfalso. step in H; simpobs. inv H.
+    - simpobs. constructor.
+      specialize (itree_eta t1) as Ht1. simpobs. 
+      sinv H. 
+      + simpobs; easy.  
+      + eapply IHeqitF; eauto. rewrite <- tau_eutt. step. 
+      rewrite x, <- H1. now constructor. 
+    - simpobs. constructor. eapply IHeqitF; eauto.
   Qed.
 
   Lemma eventless_div : forall (R : Type) (t : itree E R),
       eventless t -> all_infinite t -> t ≈ ITree.spin.
   Proof.
-    intros R. pcofix CIH. intros.
-    pinversion H0.
-    - specialize (itree_eta t) as Ht. rewrite <- H2 in Ht.
-      rewrite Ht in H1. pinversion H1.
-    - pfold. red. cbn. rewrite <- H.
-      red in H0. rewrite <- H in H0.
+    intros R. coinduction c CIH. intros.
+      sinv H.
+    - specialize (itree_eta t) as Ht. simpobs. 
+      rewrite Ht in H0. sinv H0.
+    - icbn. simpobs. 
+      red in H0. step in H0; simpobs; inv H0. 
       constructor.
-      right. apply CIH; auto.
-      specialize (itree_eta t) as Ht. rewrite <- H in Ht.
-      rewrite Ht in H1. punfold H1. red in H1. cbn in H1.
-      inversion H1. subst. pclearbot. auto.
+      apply CIH; auto. 
   Qed.
 
   Lemma eventless_ret : forall (R : Type) (t : itree E R) (r : R),
@@ -475,17 +501,16 @@ Section ITreeDijkstra.
   Proof.
     intros R t r.
     intros. induction H0; auto. rewrite H0 in H.
-    pinversion H.
+    sinv H.
   Qed.
 
   Lemma eqitE_imp_eutt : forall (E : Type -> Type) (R1 R2 : Type) (RR : R1 -> R2 -> Prop)
                                 (t1 : itree E R1) (t2 : itree E R2),
       eqitE RR t1 t2 -> eutt RR t1 t2.
   Proof.
-    intros E1 R1 R2 RR. pcofix CIH.
-    intros t1 t2 Heq. pfold. punfold Heq.
-    red. red in Heq. induction Heq; auto with itree.
-    pclearbot. constructor. right. apply CIH. auto.
+    intros E1 R1 R2 RR. coinduction c CIH.
+    intros t1 t2 Heq. icbn. step in Heq. 
+    induction Heq; auto with itree.
   Qed.
 
   Lemma eqitE_imp_eventlessl : forall (E1 E2 : Type -> Type) (R1 R2 : Type)
@@ -493,11 +518,10 @@ Section ITreeDijkstra.
                                       (t1 : itree E1 R1) (t2 : itree E2 R2),
       eqitE RR t1 t2 -> eventless t1.
   Proof.
-    intros E1 E2 R1 R2 RR. pcofix CIH.
-    intros. punfold H0. red in H0.
-    pfold. red. induction H0; eauto with itree.
-    pclearbot.
-    constructor. right. eapply CIH; eauto.
+    intros E1 E2 R1 R2 RR. coinduction c CIH.
+    intros. step in H. 
+    icbn. induction H; eauto with itree.
+    constructor. apply (CIH t0 (ITreeDefinition.go ot2)). now step. 
   Qed.
 
   Lemma eqitE_imp_eventlessr : forall (E1 E2 : Type -> Type) (R1 R2 : Type)
@@ -505,18 +529,17 @@ Section ITreeDijkstra.
                                       (t1 : itree E1 R1) (t2 : itree E2 R2),
       eqitE RR t1 t2 -> eventless t2.
   Proof.
-    intros E1 E2 R1 R2 RR. pcofix CIH.
-    intros. punfold H0. red in H0.
-    pfold. red. induction H0; eauto with itree.
-    pclearbot.
-    constructor. right. eapply CIH; eauto.
+    intros E1 E2 R1 R2 RR. coinduction c CIH.
+    intros. step in H.
+    icbn. induction H; eauto with itree.
+    constructor. apply (CIH (ITreeDefinition.go ot1) t0). now step. 
   Qed.
 
   Lemma eventless_spin : forall (E1 : Type -> Type) (R : Type),
       eventless (@ITree.spin E1 R).
   Proof.
-    intros E1 R. pcofix CIH. pfold. red. cbn. constructor.
-    right. auto.
+    intros E1 R. coinduction c CIH. icbn. cbn. constructor.
+    auto.
   Qed.
 
   CoFixpoint remove_events' {E1 E2 : Type -> Type} {A : Type}
@@ -533,10 +556,10 @@ Section ITreeDijkstra.
                                          (t : itree E1 A),
       eventless t -> @equivE E1 E2 A t (remove_events t).
   Proof.
-    intros E1 E2 A. pcofix CIH. intros.
-    pfold. red. pinversion H0.
+    intros E1 E2 A. coinduction c CIH. intros.
+    icbn. sinv H.
     - cbn. unfold remove_events. rewrite <- H1. cbn. auto with itree.
-    - unfold remove_events. rewrite <- H. cbn. constructor. right. apply CIH.
+    - unfold remove_events. rewrite <- H0. cbn. constructor. apply CIH.
       auto.
   Qed.
 
@@ -544,46 +567,54 @@ Section ITreeDijkstra.
                                          (t : itree E1 A),
       eventless (@remove_events E1 E2 A t).
   Proof.
-    intros E1 E2 A. pcofix CIH. intros.
-    pfold. red. unfold remove_events. destruct (observe t) eqn : Heq.
+    intros E1 E2 A. coinduction c CIH. intros.
+    icbn. unfold remove_events. destruct (observe t) eqn : Heq.
     - cbn. constructor.
-    - cbn. constructor. right. apply CIH.
-    - cbn. constructor. left. apply pacobot1, eventless_spin.
+    - cbn. constructor. apply CIH.
+    - cbn. constructor. do 2 step. apply eventless_spin. 
   Qed.
 
   Lemma delay_eventless : forall (A : Type) (d : Delay A),
       eventless d.
   Proof.
-    intros A. pcofix CIH. intros.
-    pfold. red. destruct (observe d); auto with itree.
+    intros A. coinduction c CIH. intros.
+    icbn. destruct (observe d); auto with itree.
     destruct e.
   Qed.
 
-  (* TODO need to get this done at some point*)
   Lemma eqitE_inv_Tau : forall (E1 E2 : Type -> Type) (R1 R2 : Type) (RR : R1 -> R2 -> Prop)
             (t1 : itree E1 R1) (t2 : itree E2 R2),
             eqitE RR (Tau t1) (Tau t2) -> eqitE RR t1 t2.
   Proof.
     intros E1 E2 R1 R2 RR.
 
-    pcofix CIH. intros.
-    punfold H0. red in H0. simpl in H0.
-    pfold. red. remember (TauF t1) as tt1.
-    remember (TauF t2) as tt2. genobs t1 ot1.
-    genobs t2 ot2. induction H0; try discriminate.
-    - pclearbot. injection Heqtt1 as Heqtt1. injection Heqtt2 as Heqtt2. subst.
-      punfold H. red in H. auto. eapply eqitE_monot; eauto.
-      intros. pclearbot. left. eapply paco2_mon; try apply PR. intros. contradiction.
-   Abort.
+    coinduction c CIH. intros. icbn. 
+    intros.
+    step in H. 
+    remember (TauF t1) as ot1. 
+    remember (TauF t2) as ot2. 
+    revert t1 t2 Heqot1 Heqot2. cbn in H. 
+    induction H; intros t1' t2' Heqot1 Heqot2; try easy; subst.
+    - inv Heqot1; inv Heqot2. now step.  
+    - inv H; inv Heqot1; simpobs. 
+      + constructor. now apply IHeqitEF. 
+      + constructor. now apply IHeqitEF.
+      + now do 2 step. 
+    - inv H; inv Heqot2; simpobs. 
+      + constructor. now apply IHeqitEF. 
+      + now do 2 step. 
+      + constructor. now apply IHeqitEF. 
+  Qed. 
+
 
   Lemma inv_remove_events : forall (E1 E2 : Type -> Type) (R : Type)
                                    (t1 : itree E1 R) (t2 : itree E2 R),
       eventless t1 -> eventless t2 -> @remove_events E1 E2 R t1 ≈ @remove_events E2 E2 R t2 ->
       equivE t1 t2.
   Proof.
-    intros E1 E2 R. pcofix CIH.
+    intros E1 E2 R. coinduction c CIH.
     intros t1 t2 Hev1 Hev2 Heutt. pfold. red.
-    punfold Heutt. unfold_eqit. dependent induction Heutt; subst.
+    step in Heutt. unfold_eqit. dependent induction Heutt; subst.
     - unfold remove_events in x0, x.
       destruct (observe t1); destruct (observe t2); try discriminate.
       constructor. cbn in *. injection x0. injection x. intros. subst. auto.
@@ -591,7 +622,7 @@ Section ITreeDijkstra.
       destruct (observe t1) eqn : Heq1; destruct (observe t2) eqn : Heq2; try discriminate.
       + cbn in *. constructor.
         injection x0. injection x. intros. subst. pclearbot.
-        right. apply CIH; auto.
+        apply CIH; auto.
         * specialize (itree_eta t1) as Ht1. rewrite Heq1 in Ht1.
           assert (t ≈ t1).
           { rewrite Ht1. rewrite tau_eutt. reflexivity. }
@@ -600,13 +631,13 @@ Section ITreeDijkstra.
           assert (t0 ≈ t2).
           { rewrite Ht2. rewrite tau_eutt. reflexivity. }
           rewrite H. auto.
-      + pinversion Hev2.
+      + sinv Hev2.
         * rewrite Heq2 in H0. discriminate.
         * rewrite Heq2 in H. discriminate.
-      + pinversion Hev1.
+      + sinv Hev1.
         * rewrite Heq1 in H0. discriminate.
         * rewrite Heq1 in H. discriminate.
-      + pinversion Hev1.
+      + sinv Hev1.
         * rewrite Heq1 in H0. discriminate.
         * rewrite Heq1 in H. discriminate.
     - unfold remove_events in *. destruct (observe t1); cbn in x0; discriminate.
@@ -619,7 +650,7 @@ Section ITreeDijkstra.
            rewrite  H. auto.
         * unfold remove_events. rewrite x. auto.
       + exfalso. specialize (itree_eta t1) as Ht1. rewrite Heq in Ht1.
-        rewrite Ht1 in Hev1. pinversion Hev1.
+        rewrite Ht1 in Hev1. sinv Hev1.
     - unfold remove_events in x. destruct (observe t2) eqn : Heq; cbn in *; try discriminate.
       + injection x as x. constructor.
         apply IHHeutt; auto.
@@ -629,7 +660,7 @@ Section ITreeDijkstra.
           rewrite H. auto.
         * unfold remove_events. rewrite x. auto.
       + exfalso. specialize (itree_eta t2) as Ht2. rewrite Heq in Ht2.
-        rewrite Ht2 in Hev2. pinversion Hev2.
+        rewrite Ht2 in Hev2. sinv Hev2.
   Qed.
 
   Lemma remove_events_eqitE : forall (E1 E2 E3 E4 : Type -> Type) (R1 R2 : Type)
@@ -637,10 +668,10 @@ Section ITreeDijkstra.
                                       (t1 : itree E1 R1) (t2 : itree E2 R2),
       eqitE RR t1 t2 -> eqitE RR (@remove_events E1 E3 R1 t1) (@remove_events E2 E4 R2 t2).
   Proof.
-    intros E1 E2 E3 E4 R1 R2 RR. pcofix CIH. intros.
-    punfold H0. red in H0. pfold. red. unfold remove_events.
+    intros E1 E2 E3 E4 R1 R2 RR. coinduction c CIH. intros.
+    step in H0. red in H0. icbn. unfold remove_events.
     induction H0; cbn; auto with itree.
-    pclearbot. constructor. right. apply CIH; auto.
+    constructor. apply CIH; auto.
   Qed.
 
   Lemma eqitE_trans : forall (E1 E2 E3 : Type -> Type) (R : Type)
@@ -670,10 +701,10 @@ Section ITreeDijkstra.
                             (t1 : itree E1 R) (t2 : itree E2 R),
       equivE t1 t2 -> equivE t2 t1.
   Proof.
-    intros E1 E2 R. pcofix CIH. intros.
-    punfold H0. red in H0. pfold. red.
+    intros E1 E2 R. coinduction c CIH. intros.
+    step in H0. red in H0. pfold. red.
     induction H0; eauto with itree.
-    pclearbot. constructor. right. apply CIH; auto.
+    constructor. apply CIH; auto.
   Qed.
 
 
@@ -772,9 +803,9 @@ Section RetBindCounter.
       unfold p. cbn. reflexivity.
     }
     apply Hcontra in H. clear Hcontra. basic_solve.
-    - unfold p in H0. cbn in H0. pinversion H0.
-    - clear H0. pinversion H; try apply all_infiniteF_mono'. ddestruction.
-      specialize (H1 tt). punfold H1; try apply all_infiniteF_mono'.
+    - unfold p in H0. cbn in H0. sinv H0.
+    - clear H0. sinv H; try apply all_infiniteF_mono'. ddestruction.
+      specialize (H1 tt). step in H1; try apply all_infiniteF_mono'.
       inv H1.
   Qed.
 
