theories/Interp/RecursionFacts.v
@@ -85,12 +85,12 @@ Proof.
   bcoinduction. intros.
   rewrite !unfold_interp_mrec.
   step in H. inv H; eauto with itree. 
-  - taus. now apply cih. 
+  - taus. now apply CIH. 
   - cbn. destruct e.
-    + taus. apply cih.
+    + taus. apply CIH.
       ebind. intros; subst.  
     do 2 step. apply REL. 
-    + constructor. intro. step. taus. apply cih.
+    + constructor. intro. step. taus. apply CIH.
     apply REL.   
 Qed.
 
@@ -104,13 +104,13 @@ Proof.
   destruct (observe t); cbn;
     [| |destruct e]; cbn. 
   - apply reflexivity.
-  - taus. fold_subst. apply cih. 
+  - taus. fold_subst. apply CIH. 
   - to_mon. taus. fold_subst. 
     rewrite <- bind_bind.
-    apply cih.  
+    apply CIH.  
   - constructor. intro. fold_subst. 
     rewrite bind_ret_l, bind_tau. 
-    step. taus. apply cih.   
+    step. taus. apply CIH.   
 Qed.
 
 Theorem interp_mrec_trigger {U} (a : (D +' E) U) :
@@ -133,13 +133,13 @@ Proof.
   rewrite unfold_interp_mrec, unfold_interp.
   destruct (observe c0); [| |destruct e]; simpl; eauto with paco.
   - now taur. 
-  - taus. apply cih. 
+  - taus. apply CIH. 
   - taus. rewrite interp_mrec_bind. unfold mrec.
-  ebind. intros; subst. apply cih. 
+  ebind. intros; subst. apply CIH. 
   - to_mon. rewrite tau_euttge. 
     unfold ITree.trigger.  rewrite bind_vis.
     constructor. intro. 
-    rewrite bind_ret_l. rewrite tau_euttge. apply cih. 
+    rewrite bind_ret_l. rewrite tau_euttge. apply CIH. 
 Qed.
 
 Theorem mrec_as_interp {T} (d : D T) :
@@ -164,21 +164,21 @@ Proof.
   rewrite (itree_eta t); destruct (observe t).
   - rewrite 2 unfold_interp_mrec; now taul. 
   - rewrite unfold_interp, 2 unfold_interp_mrec. 
-    taus. apply cih. 
+    taus. apply CIH. 
   - rewrite interp_vis.
     rewrite (unfold_interp_mrec _ (Vis _ _)).
     destruct e; cbn; to_mon. 
     + rewrite 2 interp_mrec_bind.
       taus. 
       ebind; intros; subst. 
-      rewrite unfold_interp_mrec; cbn; apply cih. 
+      rewrite unfold_interp_mrec; cbn; apply CIH. 
     + unfold inr_, Handler.Inr_sum1_Handler, Handler.Handler.inr_, Handler.Handler.htrigger.
       rewrite bind_trigger, unfold_interp_mrec; cbn; to_mon.
       rewrite tau_euttge.
       constructor.
       intros. step. taus. 
       rewrite unfold_interp_mrec; cbn.
-      apply cih. 
+      apply CIH. 
 Qed.
 
 End Facts.
@@ -196,7 +196,7 @@ Proof.
   rewrite 2 unfold_interp_mrec.
   step in Ht; induction Ht; cbn. 
   3: { destruct e; constructor. 
-    + apply cih. ebind. apply Hfg.  
+    + apply CIH. ebind. apply Hfg.  
       intros ? _ []. apply REL. 
     + intros; step; taus. eauto with paco itree.
   }
@@ -240,7 +240,7 @@ Proof.
   rewrite 2 unfold_interp_mrec.
   step in Ht; induction Ht; try easy; cbn. 
   3: { destruct e; constructor. 
-    + apply cih. ebind. apply Hfg.  
+    + apply CIH. ebind. apply Hfg.  
       intros ? _ []. apply REL. 
     + intros; step; taus. eauto with paco itree.
   }
