theories/Props/Leaf.v
@@ -309,12 +309,12 @@ Lemma has_post_of_Leaf {E R} (Q : R -> Prop) :
   (forall r, r ∈ t -> Q r) ->
   t ≈⟨ fun x _ => Q x ⟩ t.
 Proof.
-  icoinduction c cih. intros t Hpost.
+  icoinduction c CIH. intros t Hpost.
   setoid_rewrite (itree_eta t) in Hpost.
   desobs t Ht.
   - constructor. apply Hpost, Leaf_Ret.
-  - constructor. apply cih. intros. apply Hpost. apply Leaf_Tau. exact H.
-  - constructor. intros. apply cih. intros. eapply Hpost. eapply Leaf_Vis. exact H.
+  - constructor. apply CIH. intros. apply Hpost. apply Leaf_Tau. exact H.
+  - constructor. intros. apply CIH. intros. eapply Hpost. eapply Leaf_Vis. exact H.
 Qed.
 
 Lemma has_post_Leaf_equiv {E R} (t: itree E R) Q:
@@ -426,30 +426,30 @@ Qed.
 Lemma Leaf_interp_subtree_inv {E F R} (h: E ~> itree F) (t u: itree E R):
   subtree u t -> has_post (interp h u) (fun x : R => x ∈ t).
 Proof.
-  revert t u. unfold has_post. bcoinduction c cih; intros * Hsub.
+  revert t u. unfold has_post. bcoinduction c CIH; intros * Hsub.
   rewrite (itree_eta u) in Hsub.
   rewrite unfold_interp.
   desobs u Hu; clear u Hu; cbn.
   - constructor. eapply subtree_image; eauto. apply Leaf_Ret.
-  - constructor. apply cih. apply SubtreeTau, Hsub.
+  - constructor. apply CIH. apply SubtreeTau, Hsub.
   - to_mon. eapply eqit_bind_chain. reflexivity.
     intros u _ <-.
-    taus. apply cih. eapply SubtreeVis, Hsub. reflexivity.
+    taus. apply CIH. eapply SubtreeVis, Hsub. reflexivity.
 Qed.
 
 Lemma Leaf_interp_state_subtree_inv {E F S R} (h: E ~> Monads.stateT S (itree F))
   (t u: itree E R) (s: S):
   subtree u t -> has_post (interp_state h u s) (fun x => snd x ∈ t).
 Proof.
-  revert t u s. unfold has_post. bcoinduction c cih; intros * Hsub.
+  revert t u s. unfold has_post. bcoinduction c CIH; intros * Hsub.
   rewrite (itree_eta u) in Hsub.
   rewrite unfold_interp_state.
   desobs u Hu; clear u Hu; cbn.
   - constructor. eapply subtree_image; eauto. apply Leaf_Ret.
-  - constructor. apply cih. apply SubtreeTau, Hsub.
+  - constructor. apply CIH. apply SubtreeTau, Hsub.
   - to_mon. eapply eqit_bind_chain. reflexivity.
     intros [u1 u2] _ <-; cbn.
-    taus. apply cih. eapply SubtreeVis, Hsub. reflexivity.
+    taus. apply CIH. eapply SubtreeVis, Hsub. reflexivity.
 Qed.
 
 End Subtree.
